Cyclers is based on Model now

Busybeaver/TM/Model/ClosedSet.lean
@@ -11,6 +11,33 @@ structure ClosedSet (m : M) (base: Config M → Prop) (I: Config M) where
 
 namespace ClosedSet
 
+def offset {m : M} {p : Config M → Prop} {I N : Config M}
+    (closed : ClosedSet m p I) (hN : p N) : ClosedSet m p N :=
+  ⟨closed.closed, ⟨⟨N, hN⟩, .refl⟩⟩
+
+lemma nonHalting {m : M} {p : Config M → Prop} {I : Config M}
+    (inst : ClosedSet m p I) : ¬halts m I := by
+  intro ⟨final, hFinal⟩
+  induction final using Nat.caseStrongRecOn generalizing I with
+  | zero =>
+      obtain ⟨F, hFL, hFR⟩ := hFinal
+      cases hFR
+      obtain ⟨⟨N, pN⟩, hN⟩ := inst.enters
+      have hIN := halts_in_base.evstep_same hFL hN
+      cases hIN
+      obtain ⟨_, hNN'⟩ := inst.closed ⟨N, pN⟩
+      exact halts_in_base.no_progress hFL hNN'
+  | ind n IH =>
+      obtain ⟨⟨N, pN⟩, hN⟩ := inst.enters
+      obtain ⟨⟨N', pN'⟩, hNN'⟩ := inst.closed ⟨N, pN⟩
+      have hIN' : I -[m]->+' N' := Machine.EvStep.trans_progress hN hNN'
+      obtain ⟨nfin, hnfin⟩ := Progress.to_multistep hIN'
+      have hnfinn := halts_in_base.within hFinal hnfin
+      have hnfinHalts := halts_in_base.preceeds hFinal hnfin hnfinn
+      refine IH _ ?_ (inst.offset pN') hnfinHalts
+      rw [Nat.succ_sub_succ_eq_sub]
+      exact Nat.sub_le n nfin
+
 end ClosedSet
 
 end TM.Model
